
\documentclass[11pt]{article}

\usepackage{ifpdf}
\ifpdf 
    \usepackage[pdftex]{graphicx}   % to include graphics
    \pdfcompresslevel=9 
    \usepackage[pdftex,     % sets up hyperref to use pdftex driver
            plainpages=false,   % allows page i and 1 to exist in the same document
            breaklinks=true,    % link texts can be broken at the end of line
            colorlinks=true,
            pdftitle=My Document
            pdfauthor=My Good Self
           ]{hyperref} 
    \usepackage{thumbpdf}
\else 
    \usepackage{graphicx}       % to include graphics
    \usepackage{hyperref}       % to simplify the use of \href
\fi 

\title{Advanced Macroeconomic II}
\author{Nana Boateng}
\date{}

\begin{document}
\maketitle
\section{Question 1}
$u(c,l)=c^{\gamma}(1-l)^{1-\gamma}$\\

$y=Al^{\alpha}$\\

Max $u(c,l)=c^{\gamma}(1-l)^{1-\gamma}$\\

$y=Al^{\alpha}$\\

$u(l)=(Al^{\alpha})^{\gamma}(1-l)^{1-\gamma}$\\


$u^{\prime}(l)=A^{\gamma}\alpha\gamma l^{\alpha\gamma-1}(1-l)^{1-\gamma}+A^{\gamma}l^{\alpha\gamma}(\gamma-1)(1-l)^{-\gamma}=0$\\

$\alpha\gamma l^{-1}(1-l)+\gamma-1=0$\\

$\alpha\gamma l^{-1}-\alpha \gamma+\gamma-1=0$\\

$\alpha\gamma l^{-1}=\gamma(\alpha-1)+1$\\

$l^{*}=\frac{\alpha\gamma}{1+(\alpha-1)\gamma}$\\

$c^{*}=Al^{*\alpha}$

$c^{*}=A\left( \frac{\alpha\gamma}{1+(\alpha-1)\gamma}\right)$

%$u^{\prime}(l)$=$A^{\gamma}\alpha\gamma l^{\alpha \gamma-1}(1-l)^{1-\gamma}}$
%$+A^{\gamma}l^{\alpha\gamma}(\gamma-1)(1-l)^{\gamma$

\subsection{1.2}
Labor market equilibrium\\

$u(c,l_{s})=c^{\gamma}(1-l_{s})^{1-\gamma}$\\

$c=wl_{s}+\pi^{*}$\\

\section{Question 2}

Max $u(c,l_{s})= $Max  $c^{\gamma}(1-l_{s})^{}1-\gamma$\\

$c=wl_{s}+\pi^{*}$\\

$u(l_{s})=(wl_(s)+\pi^{*})^{\gamma}$\\


FOC:

$U^{\prime}(l_{s})=w\gamma(wl_{s}+\pi^{*})^{\gamma-1}(1-l_{s})^{1-\gamma}+(wl_{s}+\pi^{*})^{\gamma}(\gamma-1)(1-l_{s})^{-\gamma}$\\

$w\gamma(wl_{s}+\pi*{*})^{-1}(1-l_{s})+(\gamma-1)=0$\\

$w\gamma(1-l_{s})+(\gamma-1)(wl_{s}+\pi^{*})=0$\\

$w\gamma-w\gamma l_{s}+\gamma w l_{s}+\gamma \pi^{*}-w l_{s}-\pi^{*}=0$\\

$wl_{s}=w\gamma+\gamma\pi^{*}-\pi^{*}=\gamma w +(\gamma-1)\pi^{*}$\\

$l*{*}_{s}=\frac{\gamma w +(\gamma-1)\pi^{*}}{w}$\\

$c^{*}=wl_{s}^{*}+\pi^{*}$\\

$=\gamma w+(\gamma-1)\pi^{*}+\pi^{*}$\\

$c^{*}=\gamma(w+\pi^{*})$\\


labour and firm

$f(l_{d})=Al_{d}^{\alpha}$\\

$\pi(l_{d})=f(l_{d})-wl_{d}$


\subsection{Question 3}

Max $\pi(l_{d})= Max f(l_{d})-wl_{d}$\\

$Max Al_{d}^{\alpha}-wl_{d}$\\

FOC:\\
$\alpha Al_{d}^{\alpha-1}-w=0$\\


$\gamma(w+\pi^{*})=A\left(  \frac{w}{\alpha A} \right)^{\frac{\alpha}{\alpha-1}}$\\

$\left(\frac{w}{\gamma A}\right)^{\frac{1}{\alpha-1}}=\frac{\gamma w+(\gamma-1)\pi^{*}}{w}$\\

In a competive market $\pi^{*}=0$\\

$\gamma w=A\left(  \frac{w}{\alpha A} \right)^{\frac{\alpha}{\alpha-1}}$\\

$\left(  \frac{w}{\alpha A} \right)^{\frac{1}{\alpha-1}}=\gamma$\\

$w^{*}=\gamma^{\gamma-1}\alpha A$\\

$\pi^{*}=0$\\

$w^{*}=\alpha A \gamma^{\alpha-1}$\\

$l_{d}^{*}=\left(  \frac{w}{\alpha A} \right)^{\frac{1}{\alpha-1}}$\\

Therefore\\

$\pi^{*}=A\left(  \frac{w}{\alpha A} \right)^{\frac{1}{\alpha-1}}-w\left(  \frac{w}{\alpha A} \right)^{\frac{1}{\alpha-1}}$\\

Market clears:\\
$c^{*}=f(l_{d}^(*))$\\

$l_{d}^{*}=l_{s}^{*}$\\

\subsection{Question 4}

$\gamma(w+\pi^{*})=Al_{d}^{\alpha}$\\

$\left(  \frac{w}{\alpha A} \right)^{\frac{1}{\alpha-1}}=\frac{\gamma w +(\gamma-1)\pi^{*}}{w}$\\


\subsection{Question 5}
$l_{d}^{*}+\left(  \frac{w}{\alpha A} \right)^{\frac{1}{\alpha-1}}$\\


$=\left(  \frac{\alpha A \gamma^{\alpha-1}}{\alpha A} \right)^{\frac{1}{\alpha-1}}$\\

$l^{*}_{d}=\gamma$\\

$l^{*}_{s}=\gamma$\\


$c^{*}=A\gamma^{\alpha}$\\


\section{question 2}

Intemporal Consumption\\

$u(c_{1},c_{2})=\beta \log c_{1}+(1-\beta )\log c_{2}$\\

$p_{1}c_{1}+p_{2}c_{2}=\alpha-b_{1}+1-\alpha-b_{2}+(1+\gamma)b_{1}$\\

$p_{1}c_{1}+p_{2}c_{2}=1+\gamma b_{1}-b_{2}$\\


\subsection{1}
budget constraint is\\
$p_{1}c_{1}+p_{2}c_{2}=1+\gamma b_{1}-b_{2}$\\

\subsection{2}

Lagrangian\\
$\mathcal{L}=\beta \log c_{1}+(1-\beta )\log c_{2} +\lambda(\gamma b_{1}-b_{2}p_{1}c_{1}-p_{2}c_{2})$

\subsection{3}
FOC and Euler Equation\\

$\frac{ \partial \mathcal{L}}{\partial c_{1}}=\frac{\beta}{c_{1}}-\lambda p_{1}=0$\\


$\frac{ \partial \mathcal{L}}{\partial c_{2}}=\frac{1-\beta}{c_{2}}-\lambda p_{2}=0$\\

$\frac{ \partial \mathcal{L}}{\partial \lambda}=\gamma b_{1}-b_{2}-p_{1}c_{1}-p_{2}c_{2}=0$\\

Therefore:\\

$\frac{\beta}{c_{1}}-\lambda p_{1}=0$\\

$\frac{1-\beta}{c_{2}}-\lambda p_{2}=0$\\

$p_{1}c_{1}+p_{2}c_{2}=\gamma b_{1}-b_{2}$\\

$\frac{\beta}{c_{1}}-\lambda p_{1}=0$\\


$\frac{\beta c_{2}}{(1-\beta) c_{1}}=\frac{p_{1}}{p_{2}}$\\

$p_{1}c_{1}+p_{2}c_{2}=\gamma b_{1}-b_{2}+1$\\


\subsection{4}

Optimal Holding of bonds $b_{1},b_{2}$\\


$\beta p_{2} c_{2}=(1-\beta)p_{1}c_{1}$\\


$p_{1}c_{1}+p_{2}c_{2}=\gamma b_{1}-b_{2}+1$\\


$p_{1}c_{1}+p_{2}c_{2}=\gamma b_{1}-b_{2}+1$\\


$p_{1}c_{1}+\frac{(1-\beta)p_{1}c_{1}}{\beta}=\gamma b_{1}-b_{2}+1$\\


$p_{1}c_{1}+1-\beta)p_{1}c_{1}=\beta\gamma b_{1}-\beta b_{2}+\beta$\\


$\beta p_{2} c_{2}=(1-\beta)p_{1}c_{1}$\\


$p_{1}c_{1}=\beta\gamma b_{1}-\beta b_{2}+\beta$


$\beta p_{2} c_{2}=(1-\beta)p_{1}c_{1}$\\

$c_{1}=\frac{\beta\gamma b_{1}-\beta b_{2}+\beta}{\beta p_{1}}$\\

$c_{2}=\frac{(1-\beta)\beta\gamma b_{1}-\beta b_{2}+\beta}{\beta p_{2}}$\\



$c_{1}=\frac{\beta(\gamma b_{1}- b_{2}+1)}{\beta p_{1}}$\\


setting  $b_{2}=0$\\


$c_{2}=\frac{}{\beta p_{2}}$\\



$c_{1}=\frac{\beta+\beta\gamma b_{1}}{p_{1}}$\\

$c_{1}=\frac{\alpha-b_{1}}{p_{1}}$\\

$\alpha-b_{1}=\beta+\beta \gamma b_{1}$\\


$b_{1}=\frac{\alpha-\beta}{1+\beta\gamma}$\\

$b_{1}^{*}=\frac{\alpha-\beta}{1+\beta\gamma}$\\


$b_{1}^{*}=0$\\

\subsection{5}

Optimal value of $c_{1}$ and $c_{2}$\\


$c_{1}^{*}=\frac{\alpha-\frac{\alpha-\beta}{1+\beta \gamma}}{p_{1}}$\\


$=\frac{\alpha+\beta \gamma-\alpha +\beta}{p_{1}(1+\beta \gamma)}$\\


$c_{1}^{*}=\frac{\beta( \gamma +1)}{p_{1}(1+\beta \gamma)}$\\

$c_{2}^{*}=\frac{(1-\beta)(\beta+\gamma \beta (\frac{\alpha-\beta}{1+\beta \gamma}))}{\beta p_{2}}$\\



$c_{2}^{*}=\frac{(1-\beta)(\beta+\beta^{2}\gamma+\gamma\beta\alpha-\gamma\beta^{2})}{\beta p_{2}(1+\beta \gamma)}$\\

$c_{2}^{*}=\frac{(1-\beta)(\beta+\gamma\beta\alpha)}{\beta p_{2}(1+\beta \gamma)}$\\


$c_{2}^{*}=\frac{(1-\beta)(1+\gamma\alpha)}{ p_{2}(1+\beta \gamma)}$\\

\subsection{8}

$movement of savings rate $\\

$b_{1}^{*}=\frac{\alpha-\beta}{1+\beta \gamma}$\\

when r$\uparrow$   $b_{1}^{*}$ $\uparrow$ if $\beta >\alpha$\\

$b_{1}^{*}(\gamma)=\frac{\beta(\beta-\alpha)}{(1+\beta \gamma)^{2}}$\\

when r$\uparrow$   $b_{1}^{*}$ $\downarrow$ if $\beta <\alpha$\\

\subsection{9}

when $b_{1}^{*}=b_{2}^{*}=0$\\

$\alpha-\beta=0$\\

$\alpha=\beta$\\

\section{Question 3}
\title{Intertemporal Budget Constraints}

$b_{0},b_{1}\cdots,b_{t},b_{t+1} $are bonds\\

$w_{1}n_{1}+rb_{0}=p_{1}c_{1}$\\


$w_{2}n_{2}+rb_{0}+rb_{1}=p_{2}c_{2}$\\

$w_{3}n_{3}+rb_{0}+rb_{1}+rb_{2}=p_{3}c_{3}$\\

$\vdots$

$w_{t}n_{t}+r(b_{0}+b_{1}+b_{2}\cdots b_{t-1}) =p_{t}c_{t}$\\

\subsection{q1}
$w_{t}n_{t}+r(b_{0}+b_{1}+b_{2}\cdots b_{t-1}) =p_{t}c_{t}$\\ is the dynamic budget constraint

\subsection{q2}

$w_{1}n_{1}+rb_{0}=p_{1}c_{1}$\\


$w_{2}n_{2}+rb_{0}+rb_{1}=p_{2}c_{2}$\\



$\vdots$

$w_{T}n_{T}+r(b_{0}+b_{1}+b_{2}\cdots b_{T-1}) =p_{T}c_{T}$\\


\subsection{q3}

$w_{1}n_{1}+rb_{0}=p_{1}c_{1}$\\

$+$

$w_{2}n_{2}+rb_{0}+rb_{1}=p_{2}c_{2}$\\

$+$

$ \underline {w_{T}n_{T}+r(b_{0}+b_{1}+b_{2}\cdots b_{T-1}) =p_{T}c_{T} }$\\

%\underline

$\sum_{t=1}^{T}w_{t}n_{t}+rTb_{0}+r(T-1)b_{1}+\cdots+rb_{T-1}=\sum_{t=1}^{T}p_{t}c_{t}$

\section{Question 4 }

\title{Intertemporal Crusoe}\\


$u(c,l)=\ln(c_{1})+\ln(1-l_{1})+\beta \left(\ln c_{2}+\ln(1-l_{2})\right)$\\


\subsection{q1}
Robinson's Constraint

$c_{1}=2l_{1}-s$\\

$c_{2}=l_{2}+R-s$\\

\subsection{q2}
Robinson's Tax Problem\\

Max $u(c,l)=\ln(c_{1})+\ln(1-l_{1})+ \left(\ln c_{2}+\ln(1-l_{2})\right)$\\

$c_{1}+c_{2}=2l_{1}+l_{2}-s+Rs$\\


\subsection{q3}
Euler Equation\\

$\mathcal{L}=\ln c_{1}+\ln(1-l_{1}) +\ln c_{2}+\ln(1-l_{2}) +\lambda \left(2l_{1}+l_{2}-s+Rs-c_{1}-c_{2} \right)$\\




$\frac{\partial \mathcal{L}}{\partial c_{1}}=\frac{1}{c_{1}}-\lambda=0$\\


$\frac{\partial \mathcal{L}}{\partial c_{2}}=\frac{1}{c_{2}}-\lambda=0$\\


$\frac{\partial \mathcal{L}}{\partial \lambda}=2l_{1}+l_{2}-s+Rs-c_{1}-c_{2}=0$\\

Euler Equation of Consumption\\

$\frac{c_{2}}{c_{2}}=1$\\

$2l_{1}+l_{2}-s+Rs=c_{1}+c_{2}$\\

$\frac{\partial \mathcal{L}}{\partial l_{1}}=\frac{-1}{1-l_{1}}+2\lambda=0$\\


$\frac{\partial \mathcal{L}}{\partial l_{1}}=\frac{-1}{1-l_{2}}+\lambda=0$\\


$\frac{\partial \mathcal{L}}{\partial \lambda}=2l_{1}+l_{2}-s+Rs-c_{1}-c_{2}=0$

leisure Euler Equation

$\frac{1-l_{2}}{1-l_{2}}=2$\\

$2l_{1}+l_{2}-s+Rs=c_{1}+c_{2}$\\


$\lambda=\frac{1}{c_{1}}$\\

$\lambda=\frac{1}{c_{2}}$\\

$\lambda=\frac{1}{2(1-l_{1})}$\\


$\lambda=\frac{1}{(1-1_{2})}$\\

Eulers Intemporal between consumption and leisure\\

$\frac{c_{2}}{c_{1}} \times \frac {1-l_{2}}{1-l_{2}}=2$


\subsection{q4}

$1-l_{2}=2-l_{1}$\\

$c_{2}=c_{1}$\\

$2l_{1}+l_{2}-s+Rs=c_{1}+c_{2}$\\

$1+l_{2}=-1+2l_{2}$\\

$c_{2}=c_{1}$\\

$2l_{1}-1+2l_{1}-s+Rs=c_{1}$\\


$l_{2}=-1+2l_{2}$\\

$c_{2}=c_{1}$\\

$24_{1}-1-s+Rs-1=2c_{1}$\\

$c_{1}=2l_{1}-s$\\





\end{document}  
